test-suite/reify_prop.v
@@ -1,5 +1,147 @@
+Require Import Coq.quote.Quote.
 Require Import Reify Bvector.
+Require Import List.
+Notation dyn x := (@mkDynamic _ x).
+Require Import Program.
+Print End_idx.
+Inductive prop : Set :=
+| prop_true | prop_false | prop_conj (A B : prop) | prop_disj (A B : prop)
+| prop_impl (A B : prop) | prop_var (n : index).
 
-Goal True.
+Definition find_var {A:Type} (def : prop) (i : index) (v : varmap A) :=
+  prop_var i.
+
+Definition prop_map :=
+  [(dyn True, dyn prop_true);
+   (dyn False, dyn prop_false);
+   (dyn and, dyn prop_conj);
+   (dyn or, dyn prop_disj);
+   (dyn impl, dyn prop_impl);
+   (dyn varmap_find, dyn (@find_var))
+  ].
+
+Fixpoint interp (v : varmap Prop) (p : prop) : Prop :=
+  match p with
+    | prop_true => True
+    | prop_false => False
+    | prop_conj P Q => and (interp v P) (interp v Q)
+    | prop_disj P Q => or (interp v P) (interp v Q)
+    | prop_impl P Q => impl (interp v P) (interp v Q)
+    | prop_var idx => varmap_find True idx v
+  end.
+Require Import ZArith.
+Inductive expr : Set :=
+| Evar (i : index)
+| Emult (e e' : expr)
+| Eplus (e e' : expr)
+| Ecst (z : Z).
+
+Definition find_vare {A:Type} (def : expr) (i : index) (v : varmap Z) :=
+  Evar i.
+
+Open Scope Z_scope.
+
+Fixpoint interpe (v : varmap Z) (p : expr) : Z :=
+  match p with
+    | Evar i => varmap_find 0 i v
+    | Emult e e' => (interpe v e) * (interpe v e')
+    | Eplus e e' => (interpe v e) + (interpe v e')
+    | Ecst z => z
+  end.
+
+
+Definition expr_map :=
+  [(dyn Z, dyn expr);
+   (dyn Z0, dyn (Ecst Z0));
+   (dyn Zmult, dyn Emult);
+   (dyn Zplus, dyn Eplus);
+   (dyn 2, dyn (Ecst 2));
+   (dyn varmap_find, dyn (@find_vare))
+  ].
+
+Ltac reifye :=
+  match goal with
+    |- ?T => 
+      let vars := fresh "vars" in let goal' := fresh "goal'" in
+      let l := eval cbv delta [expr_map] in expr_map in
+        reify vars goal' Z 0 l T;
+        match eval red in goal' with
+          ?x = ?y => change (interpe vars x = interpe vars y)
+        end
+  end.
+
+Goal forall x y, x * y = x * y. 
+intros. reifye. Admitted.
+
+Fixpoint test (zs : list Z) : Z :=
+  match zs with
+    | nil => 2
+    | x :: l => let y := test l in
+      (x * y) + (y * x)
+  end.
+
+Goal forall x1 x2 x3, test (x1 :: x2 :: x3 :: nil) = test (x3 :: x2 :: x1 :: nil).
+Proof.
+  intros. unfold test.
+  Time reifye. 
+Admitted.
+
+Goal forall x1 x2 x3 x4 x5, test (x1 :: x2 :: x3 :: x4 :: x5 :: nil) = 
+test (x5 :: x4 :: x3 :: x2 :: x1 :: nil).
+Proof.
+  intros. unfold test.
+  Time reifye.
+Admitted.
+
+
+Goal forall x1 x2 x3 x4 x5 x1' x2' x3' x4' x5', 
+  test (x1 :: x2 :: x3 :: x4 :: x5 :: x1' :: x2' :: x3' :: x4' :: x5' :: nil) = 
+test (x5' :: x4' :: x3' :: x2' :: x1' :: x5 :: x4 :: x3 :: x2 :: x1 :: nil).
+Proof.
+  intros. unfold test.
+
+Set Printing Depth 20.
+
+Ltac reifye ::=
+  match goal with
+    |- ?T => 
+      let vars := fresh "vars" in let goal' := fresh "goal'" in
+      let l := eval cbv delta [expr_map] in expr_map in
+        reify vars goal' Z 0 l T; unfold find_vare in goal' end.
+  Time reifye. idtac.
+Admitted.
+
+Goal forall x1 x2 x3 x4 x5 x1' x2' x3' x4' x5' x1'' x2'' x3'' x4'' x5'', 
+  test (x1 :: x2 :: x3 :: x4 :: x5 :: x1' :: x2' :: x3' :: x4' :: x5' :: x1'' :: x2'' :: x3'' :: x4'' :: x5'' :: nil) = 
+  test (x5'' :: x4'' :: x3'' :: x2'' :: x1'' :: x5' :: x4' :: x3' :: x2' :: x1' :: x5 :: x4 :: x3 :: x2 :: x1 :: nil).
+Proof.
+  intros. unfold test.
+
+Set Printing Depth 20.
+
+Ltac reifye ::=
+  match goal with
+    |- ?T => 
+      let vars := fresh "vars" in let goal' := fresh "goal'" in
+      let l := eval cbv delta [expr_map] in expr_map in
+        reify vars goal' Z 0 l T; unfold find_vare in goal' end.
+  Time reifye. idtac.
+Admitted.
+
+
+Goal forall P : Prop, P /\ True.
+intros P.
+match goal with
+  |- ?T => 
+    let l := eval cbv delta [prop_map] in prop_map in
+      idtac l;
+    reify vars goal Prop True l T
+end. subst goal. simpl.
+exact I.
+Defined.
+
+match goal with
+  |- ?T => varify vars goal Prop True T; change goal
+end. subst goal.
 exact I.
 Defined.
